subst_help.v
@@ -1,10 +1,11 @@
 
 From Coq.Lists Require Import List.
 From mathcomp Require Import ssreflect ssrfun ssrbool seq eqtype ssrnat.
-From istari Require Import source subst_src rules_src basic_types help.
+From istari Require Import source subst_src rules_src basic_types
+     subst_help0 help0 help.
 From istari Require Import Sigma Tactics
      Syntax Subst SimpSub Promote Hygiene
-     ContextHygiene Equivalence Rules Defined.
+     ContextHygiene Equivalence Rules Defined PageType.
 
 Lemma subst_world: forall s,
     subst s world = world.
@@ -36,6 +37,7 @@ Lemma subst_subseq: forall w1 w2 l1 l2 s,
    simpsub_bigs.
    auto.
  Qed.
+Hint Rewrite subst_subseq : core subst1.
 
 Lemma subst_laters: forall s A, (subst s (laters A)) = (laters (subst s A)).
   intros. unfold laters. unfold plus. rewrite subst_rec. rewrite subst_sigma.
@@ -48,26 +50,6 @@ Lemma subst_store: forall w l s, subst s (store w l) = store (subst s w) (subst 
 Hint Rewrite subst_store: core subst1.
 
 
- Lemma subst_move: forall A l1 l2 s, (subst s (move A l1 l2)) = move A (subst s l1) (subst s l2).
-   intros. induction A; unfold make_subseq_trans;
-unfold leq_trans_fn_app; unfold leq_trans_fn; simpsub_big; simpl; auto.
-   { unfold make_subseq_trans;
-unfold leq_trans_fn_app; unfold leq_trans_fn; simpsub_big; simpl; auto.
-}
-   { unfold make_subseq_trans;
-unfold leq_trans_fn_app; unfold leq_trans_fn; simpsub_big; simpl; auto.
-}
-   { unfold make_subseq_trans;
-       unfold lt_trans_fn_app; unfold leq_trans_fn_app;
-         unfold leq_trans_fn; simpsub_big; simpl; auto.
-}
- Qed.
-
-Hint Rewrite subst_move: core subst1.
-
-Lemma subst_moveapp s A l1 l2 m1 m2 : (subst s (move_app A l1 l2 m1 m2)) =
-                              move_app A (subst s l1) (subst s l2) (subst s m1) (subst s m2).
-   unfold move_app. simpsub_big. auto. Qed.
 
 Lemma subst_consb w l x s: @ subst obj s (cons_b w l x) =
                            cons_b (subst s w) (subst s l) (subst s x).
@@ -88,28 +70,11 @@ Lemma subst_make_subseq_trans: forall s a b c d e, (subst s (make_subseq_trans a
 Hint Rewrite subst_make_subseq_trans: core subst1.
 Hint Rewrite <- subst_make_subseq_trans : inv_subst.
 
-Lemma subst_lttp: forall s,
-    @ subst obj s (lttp) = lttp.
-  intros. unfold lttp.
-  simpsub. rewrite subst_leqtp. unfold nsucc. simpsub. simpl.
-  rewrite subst_leqtp. auto. Qed.
-Hint Rewrite subst_leqtp: core subst1.
-
-Lemma subst_leq: forall s n1 n2,
-    @ subst obj s (leq_t n1 n2) =  leq_t (subst s n1) (subst s n2).
-  intros. unfold leq_t.  repeat rewrite subst_app. auto. 
-Qed.
-
-Lemma subst_lt: forall s n1 n2,
-    subst s (lt_t n1 n2) = lt_t (subst s n1) (@ subst obj s n2).
-  intros. repeat rewrite subst_app. rewrite subst_lttp. auto. Qed. 
 
 Lemma subst_nth: forall s m1 m2, (subst s (nth m1 m2)) = (nth (subst s m1) (subst s m2)). intros. unfold nth. simpsub. auto. Qed.
 
 Lemma subst_make_subseq: forall s, (subst s make_subseq) = make_subseq.
   intros. unfold make_subseq. simpsub. auto. Qed.
 
-Hint Rewrite subst_subseq subst_leq subst_lttp subst_lt
-     subst_pw subst_world subst_nth subst_laters subst_make_subseq subst_ltb
-subst_moveapp
-.
+Hint Rewrite subst_subseq 
+     subst_pw subst_world subst_nth subst_laters subst_make_subseq subst_ltb : core subst1.
